Partial conversion of UNITY to Isar new-style theories

src/HOL/UNITY/Simple/Reachability.thy
@@ -8,65 +8,367 @@ Reachability in Graphs
 From Chandy and Misra, "Parallel Program Design" (1989), sections 6.2 and 11.3
 *)
 
-Reachability = Detects + 
+theory Reachability = Detects + Reach:
 
 types  edge = "(vertex*vertex)"
 
 record state =
-  reach :: vertex => bool
-  nmsg  :: edge => nat
+  reach :: "vertex => bool"
+  nmsg  :: "edge => nat"
 
-consts REACHABLE :: edge set
-       root :: vertex
-       E :: edge set
-       V :: vertex set
+consts REACHABLE :: "edge set"
+       root :: "vertex"
+       E :: "edge set"
+       V :: "vertex set"
 
 inductive "REACHABLE"
-  intrs
-   base "v : V ==> ((v,v) : REACHABLE)"
-   step "((u,v) : REACHABLE) & (v,w) : E ==> ((u,w) : REACHABLE)"
+  intros
+   base: "v : V ==> ((v,v) : REACHABLE)"
+   step: "((u,v) : REACHABLE) & (v,w) : E ==> ((u,w) : REACHABLE)"
 
 constdefs
-  reachable :: vertex => state set
+  reachable :: "vertex => state set"
   "reachable p == {s. reach s p}"
 
-  nmsg_eq :: nat => edge  => state set
+  nmsg_eq :: "nat => edge  => state set"
   "nmsg_eq k == %e. {s. nmsg s e = k}"
 
-  nmsg_gt :: nat => edge  => state set
+  nmsg_gt :: "nat => edge  => state set"
   "nmsg_gt k  == %e. {s. k < nmsg s e}"
 
-  nmsg_gte :: nat => edge => state set
+  nmsg_gte :: "nat => edge => state set"
   "nmsg_gte k == %e. {s. k <= nmsg s e}"
 
-  nmsg_lte  :: nat => edge => state set
+  nmsg_lte  :: "nat => edge => state set"
   "nmsg_lte k  == %e. {s. nmsg s e <= k}"
 
   
 
-  final :: state set
+  final :: "state set"
   "final == (INTER V (%v. reachable v <==> {s. (root, v) : REACHABLE})) Int (INTER E (nmsg_eq 0))"
 
-rules
-    Graph1 "root : V"
+axioms
 
-    Graph2 "(v,w) : E ==> (v : V) & (w : V)"
+    Graph1: "root : V"
 
-    MA1  "F : Always (reachable root)"
+    Graph2: "(v,w) : E ==> (v : V) & (w : V)"
 
-    MA2  "[|v:V|] ==> F : Always (- reachable v Un {s. ((root,v) : REACHABLE)})"
+    MA1:  "F : Always (reachable root)"
 
-    MA3  "[|v:V;w:V|] ==> F : Always (-(nmsg_gt 0 (v,w)) Un (reachable v))"
+    MA2:  "v: V ==> F : Always (- reachable v Un {s. ((root,v) : REACHABLE)})"
 
-    MA4  "[|(v,w) : E|] ==> F : Always (-(reachable v) Un (nmsg_gt 0 (v,w)) Un (reachable w))"
+    MA3:  "[|v:V;w:V|] ==> F : Always (-(nmsg_gt 0 (v,w)) Un (reachable v))"
 
-    MA5  "[|v:V;w:V|] ==> F : Always (nmsg_gte 0 (v,w) Int nmsg_lte (Suc 0) (v,w))"
+    MA4:  "(v,w) : E ==> 
+           F : Always (-(reachable v) Un (nmsg_gt 0 (v,w)) Un (reachable w))"
 
-    MA6  "[|v:V|] ==> F : Stable (reachable v)"
+    MA5:  "[|v:V; w:V|] 
+           ==> F : Always (nmsg_gte 0 (v,w) Int nmsg_lte (Suc 0) (v,w))"
 
-    MA6b "[|v:V;w:W|] ==> F : Stable (reachable v Int nmsg_lte k (v,w))"
+    MA6:  "[|v:V|] ==> F : Stable (reachable v)"
 
-    MA7  "[|v:V;w:V|] ==> F : UNIV LeadsTo nmsg_eq 0 (v,w)"
+    MA6b: "[|v:V;w:W|] ==> F : Stable (reachable v Int nmsg_lte k (v,w))"
+
+    MA7:  "[|v:V;w:V|] ==> F : UNIV LeadsTo nmsg_eq 0 (v,w)"
+
+
+lemmas E_imp_in_V_L = Graph2 [THEN conjunct1, standard]
+lemmas E_imp_in_V_R = Graph2 [THEN conjunct2, standard]
+
+lemma lemma2:
+     "(v,w) : E ==> F : reachable v LeadsTo nmsg_eq 0 (v,w) Int reachable v"
+apply (rule MA7 [THEN PSP_Stable, THEN LeadsTo_weaken_L])
+apply (rule_tac [3] MA6)
+apply (auto simp add: E_imp_in_V_L E_imp_in_V_R)
+done
+
+lemma Induction_base: "(v,w) : E ==> F : reachable v LeadsTo reachable w"
+apply (rule MA4 [THEN Always_LeadsTo_weaken])
+apply (rule_tac [2] lemma2)
+apply (auto simp add: nmsg_eq_def nmsg_gt_def)
+done
+
+lemma REACHABLE_LeadsTo_reachable:
+     "(v,w) : REACHABLE ==> F : reachable v LeadsTo reachable w"
+apply (erule REACHABLE.induct)
+apply (rule subset_imp_LeadsTo, blast)
+apply (blast intro: LeadsTo_Trans Induction_base)
+done
+
+lemma Detects_part1: "F : {s. (root,v) : REACHABLE} LeadsTo reachable v"
+apply (rule single_LeadsTo_I)
+apply (simp split add: split_if_asm)
+apply (rule MA1 [THEN Always_LeadsToI])
+apply (erule REACHABLE_LeadsTo_reachable [THEN LeadsTo_weaken_L], auto)
+done
+
+
+lemma Reachability_Detected: 
+     "v : V ==> F : (reachable v) Detects {s. (root,v) : REACHABLE}"
+apply (unfold Detects_def, auto)
+ prefer 2 apply (blast intro: MA2 [THEN Always_weaken])
+apply (rule Detects_part1 [THEN LeadsTo_weaken_L], blast)
+done
+
+
+lemma LeadsTo_Reachability:
+     "v : V ==> F : UNIV LeadsTo (reachable v <==> {s. (root,v) : REACHABLE})"
+by (erule Reachability_Detected [THEN Detects_Imp_LeadstoEQ])
+
+
+(* ------------------------------------ *)
+
+(* Some lemmas about <==> *)
+
+lemma Eq_lemma1: 
+     "(reachable v <==> {s. (root,v) : REACHABLE}) =  
+      {s. ((s : reachable v) = ((root,v) : REACHABLE))}"
+apply (unfold Equality_def, blast)
+done
+
+
+lemma Eq_lemma2: 
+     "(reachable v <==> (if (root,v) : REACHABLE then UNIV else {})) =  
+      {s. ((s : reachable v) = ((root,v) : REACHABLE))}"
+apply (unfold Equality_def, auto)
+done
+
+(* ------------------------------------ *)
+
+
+(* Some lemmas about final (I don't need all of them!)  *)
+
+lemma final_lemma1: 
+     "(INT v: V. INT w:V. {s. ((s : reachable v) = ((root,v) : REACHABLE)) &  
+                              s : nmsg_eq 0 (v,w)})  
+      <= final"
+apply (unfold final_def Equality_def, auto)
+apply (frule E_imp_in_V_R)
+apply (frule E_imp_in_V_L, blast)
+done
+
+lemma final_lemma2: 
+ "E~={}  
+  ==> (INT v: V. INT e: E. {s. ((s : reachable v) = ((root,v) : REACHABLE))}  
+                           Int nmsg_eq 0 e)    <=  final"
+apply (unfold final_def Equality_def)
+apply (auto split add: split_if_asm)
+apply (frule E_imp_in_V_L, blast)
+done
+
+lemma final_lemma3:
+     "E~={}  
+      ==> (INT v: V. INT e: E.  
+           (reachable v <==> {s. (root,v) : REACHABLE}) Int nmsg_eq 0 e)  
+          <= final"
+apply (frule final_lemma2)
+apply (simp (no_asm_use) add: Eq_lemma2)
+done
+
+
+lemma final_lemma4:
+     "E~={}  
+      ==> (INT v: V. INT e: E.  
+           {s. ((s : reachable v) = ((root,v) : REACHABLE))} Int nmsg_eq 0 e)  
+          = final"
+apply (rule subset_antisym)
+apply (erule final_lemma2)
+apply (unfold final_def Equality_def, blast)
+done
+
+lemma final_lemma5:
+     "E~={}  
+      ==> (INT v: V. INT e: E.  
+           ((reachable v) <==> {s. (root,v) : REACHABLE}) Int nmsg_eq 0 e)  
+          = final"
+apply (frule final_lemma4)
+apply (simp (no_asm_use) add: Eq_lemma2)
+done
+
+
+lemma final_lemma6:
+     "(INT v: V. INT w: V.  
+       (reachable v <==> {s. (root,v) : REACHABLE}) Int nmsg_eq 0 (v,w))  
+      <= final"
+apply (simp (no_asm) add: Eq_lemma2 Int_def)
+apply (rule final_lemma1)
+done
+
+
+lemma final_lemma7: 
+     "final =  
+      (INT v: V. INT w: V.  
+       ((reachable v) <==> {s. (root,v) : REACHABLE}) Int  
+       (-{s. (v,w) : E} Un (nmsg_eq 0 (v,w))))"
+apply (unfold final_def)
+apply (rule subset_antisym, blast)
+apply (auto split add: split_if_asm)
+apply (blast dest: E_imp_in_V_L E_imp_in_V_R)+
+done
+
+(* ------------------------------------ *)
+
+
+(* ------------------------------------ *)
+
+(* Stability theorems *)
+lemma not_REACHABLE_imp_Stable_not_reachable:
+     "[| v : V; (root,v) ~: REACHABLE |] ==> F : Stable (- reachable v)"
+apply (drule MA2 [THEN AlwaysD], auto)
+done
+
+lemma Stable_reachable_EQ_R:
+     "v : V ==> F : Stable (reachable v <==> {s. (root,v) : REACHABLE})"
+apply (simp (no_asm) add: Equality_def Eq_lemma2)
+apply (blast intro: MA6 not_REACHABLE_imp_Stable_not_reachable)
+done
+
+
+lemma lemma4: 
+     "((nmsg_gte 0 (v,w) Int nmsg_lte (Suc 0) (v,w)) Int 
+       (- nmsg_gt 0 (v,w) Un A))  
+      <= A Un nmsg_eq 0 (v,w)"
+apply (unfold nmsg_gte_def nmsg_lte_def nmsg_gt_def nmsg_eq_def, auto)
+done
+
+
+lemma lemma5: 
+     "reachable v Int nmsg_eq 0 (v,w) =  
+      ((nmsg_gte 0 (v,w) Int nmsg_lte (Suc 0) (v,w)) Int  
+       (reachable v Int nmsg_lte 0 (v,w)))"
+apply (unfold nmsg_gte_def nmsg_lte_def nmsg_gt_def nmsg_eq_def, auto)
+done
+
+lemma lemma6: 
+     "- nmsg_gt 0 (v,w) Un reachable v <= nmsg_eq 0 (v,w) Un reachable v"
+apply (unfold nmsg_gte_def nmsg_lte_def nmsg_gt_def nmsg_eq_def, auto)
+done
+
+lemma Always_reachable_OR_nmsg_0:
+     "[|v : V; w : V|] ==> F : Always (reachable v Un nmsg_eq 0 (v,w))"
+apply (rule Always_Int_I [OF MA5 MA3, THEN Always_weaken])
+apply (rule_tac [5] lemma4, auto)
+done
+
+lemma Stable_reachable_AND_nmsg_0:
+     "[|v : V; w : V|] ==> F : Stable (reachable v Int nmsg_eq 0 (v,w))"
+apply (subst lemma5)
+apply (blast intro: MA5 Always_imp_Stable [THEN Stable_Int] MA6b)
+done
+
+lemma Stable_nmsg_0_OR_reachable:
+     "[|v : V; w : V|] ==> F : Stable (nmsg_eq 0 (v,w) Un reachable v)"
+by (blast intro!: Always_weaken [THEN Always_imp_Stable] lemma6 MA3)
+
+lemma not_REACHABLE_imp_Stable_not_reachable_AND_nmsg_0:
+     "[| v : V; w:V; (root,v) ~: REACHABLE |]  
+      ==> F : Stable (- reachable v Int nmsg_eq 0 (v,w))"
+apply (rule Stable_Int [OF MA2 [THEN Always_imp_Stable] 
+                           Stable_nmsg_0_OR_reachable, 
+            THEN Stable_eq])
+   prefer 4 apply blast
+apply auto
+done
+
+lemma Stable_reachable_EQ_R_AND_nmsg_0:
+     "[| v : V; w:V |]  
+      ==> F : Stable ((reachable v <==> {s. (root,v) : REACHABLE}) Int  
+                      nmsg_eq 0 (v,w))"
+by (simp add: Equality_def Eq_lemma2  Stable_reachable_AND_nmsg_0
+              not_REACHABLE_imp_Stable_not_reachable_AND_nmsg_0)
+
+
+
+(* ------------------------------------ *)
+
+
+(* LeadsTo final predicate (Exercise 11.2 page 274) *)
+
+lemma UNIV_lemma: "UNIV <= (INT v: V. UNIV)"
+by blast
+
+lemmas UNIV_LeadsTo_completion = 
+    LeadsTo_weaken_L [OF Finite_stable_completion UNIV_lemma]
+
+lemma LeadsTo_final_E_empty: "E={} ==> F : UNIV LeadsTo final"
+apply (unfold final_def, simp)
+apply (rule UNIV_LeadsTo_completion)
+  apply safe
+ apply (erule LeadsTo_Reachability [simplified])
+apply (drule Stable_reachable_EQ_R, simp)
+done
+
+
+lemma Leadsto_reachability_AND_nmsg_0:
+     "[| v : V; w:V |]  
+      ==> F : UNIV LeadsTo  
+             ((reachable v <==> {s. (root,v): REACHABLE}) Int nmsg_eq 0 (v,w))"
+apply (rule LeadsTo_Reachability [THEN LeadsTo_Trans], blast)
+apply (subgoal_tac
+	 "F : (reachable v <==> {s. (root,v) : REACHABLE}) Int 
+              UNIV LeadsTo (reachable v <==> {s. (root,v) : REACHABLE}) Int 
+              nmsg_eq 0 (v,w) ")
+apply simp
+apply (rule PSP_Stable2)
+apply (rule MA7)
+apply (rule_tac [3] Stable_reachable_EQ_R, auto)
+done
+
+lemma LeadsTo_final_E_NOT_empty: "E~={} ==> F : UNIV LeadsTo final"
+apply (rule LeadsTo_weaken_L [OF LeadsTo_weaken_R UNIV_lemma])
+apply (rule_tac [2] final_lemma6)
+apply (rule Finite_stable_completion)
+  apply blast
+ apply (rule UNIV_LeadsTo_completion)
+   apply (blast intro: Stable_INT Stable_reachable_EQ_R_AND_nmsg_0
+                    Leadsto_reachability_AND_nmsg_0)+
+done
+
+lemma LeadsTo_final: "F : UNIV LeadsTo final"
+apply (case_tac "E={}")
+apply (rule_tac [2] LeadsTo_final_E_NOT_empty)
+apply (rule LeadsTo_final_E_empty, auto)
+done
+
+(* ------------------------------------ *)
+
+(* Stability of final (Exercise 11.2 page 274) *)
+
+lemma Stable_final_E_empty: "E={} ==> F : Stable final"
+apply (unfold final_def, simp)
+apply (rule Stable_INT)
+apply (drule Stable_reachable_EQ_R, simp)
+done
+
+
+lemma Stable_final_E_NOT_empty: "E~={} ==> F : Stable final"
+apply (subst final_lemma7)
+apply (rule Stable_INT)
+apply (rule Stable_INT)
+apply (simp (no_asm) add: Eq_lemma2)
+apply safe
+apply (rule Stable_eq)
+apply (subgoal_tac [2] "({s. (s : reachable v) = ((root,v) : REACHABLE) } Int nmsg_eq 0 (v,w)) = ({s. (s : reachable v) = ( (root,v) : REACHABLE) } Int (- UNIV Un nmsg_eq 0 (v,w))) ")
+prefer 2 apply blast 
+prefer 2 apply blast 
+apply (rule Stable_reachable_EQ_R_AND_nmsg_0
+            [simplified Eq_lemma2 Collect_const])
+apply (blast, blast)
+apply (rule Stable_eq)
+ apply (rule Stable_reachable_EQ_R [simplified Eq_lemma2 Collect_const])
+ apply simp
+apply (subgoal_tac 
+        "({s. (s : reachable v) = ((root,v) : REACHABLE) }) = 
+         ({s. (s : reachable v) = ( (root,v) : REACHABLE) } Int
+              (- {} Un nmsg_eq 0 (v,w)))")
+apply blast+
+done
+
+lemma Stable_final: "F : Stable final"
+apply (case_tac "E={}")
+prefer 2 apply (blast intro: Stable_final_E_NOT_empty)
+apply (blast intro: Stable_final_E_empty)
+done
 
 end
 
