src/HOL/UNITY/Detects.thy
@@ -6,16 +6,78 @@
 Detects definition (Section 3.8 of Chandy & Misra) using LeadsTo
 *)
 
-Detects = WFair + Reach + 
-
+theory Detects = FP + SubstAx:
 
 consts
    op_Detects  :: "['a set, 'a set] => 'a program set"  (infixl "Detects" 60)
    op_Equality :: "['a set, 'a set] => 'a set"          (infixl "<==>" 60)
    
 defs
-  Detects_def "A Detects B == (Always (-A Un B)) Int (B LeadsTo A)"
-  Equality_def "A <==> B == (-A Un B) Int (A Un -B)"
+  Detects_def:  "A Detects B == (Always (-A Un B)) Int (B LeadsTo A)"
+  Equality_def: "A <==> B == (-A Un B) Int (A Un -B)"
+
+
+(* Corollary from Sectiom 3.6.4 *)
+
+lemma Always_at_FP: "F: A LeadsTo B ==> F : Always (-((FP F) Int A Int -B))"
+apply (rule LeadsTo_empty)
+apply (subgoal_tac "F : (FP F Int A Int - B) LeadsTo (B Int (FP F Int -B))")
+apply (subgoal_tac [2] " (FP F Int A Int - B) = (A Int (FP F Int -B))")
+apply (subgoal_tac "(B Int (FP F Int -B)) = {}")
+apply auto
+apply (blast intro: PSP_Stable stable_imp_Stable stable_FP_Int)
+done
+
+
+lemma Detects_Trans: 
+     "[| F : A Detects B; F : B Detects C |] ==> F : A Detects C"
+apply (unfold Detects_def Int_def)
+apply (simp (no_asm))
+apply safe
+apply (rule_tac [2] LeadsTo_Trans)
+apply auto
+apply (subgoal_tac "F : Always ((-A Un B) Int (-B Un C))")
+ apply (blast intro: Always_weaken)
+apply (simp add: Always_Int_distrib)
+done
+
+lemma Detects_refl: "F : A Detects A"
+apply (unfold Detects_def)
+apply (simp (no_asm) add: Un_commute Compl_partition subset_imp_LeadsTo)
+done
+
+lemma Detects_eq_Un: "(A<==>B) = (A Int B) Un (-A Int -B)"
+apply (unfold Equality_def)
+apply blast
+done
+
+(*Not quite antisymmetry: sets A and B agree in all reachable states *)
+lemma Detects_antisym: 
+     "[| F : A Detects B;  F : B Detects A|] ==> F : Always (A <==> B)"
+apply (unfold Detects_def Equality_def)
+apply (simp add: Always_Int_I Un_commute)
+done
+
+
+(* Theorem from Section 3.8 *)
+
+lemma Detects_Always: 
+     "F : A Detects B ==> F : Always ((-(FP F)) Un (A <==> B))"
+apply (unfold Detects_def Equality_def)
+apply (simp (no_asm) add: Un_Int_distrib Always_Int_distrib)
+apply (blast dest: Always_at_FP intro: Always_weaken)
+done
+
+(* Theorem from exercise 11.1 Section 11.3.1 *)
+
+lemma Detects_Imp_LeadstoEQ: 
+     "F : A Detects B ==> F : UNIV LeadsTo (A <==> B)"
+apply (unfold Detects_def Equality_def)
+apply (rule_tac B = "B" in LeadsTo_Diff)
+prefer 2 apply (blast intro: Always_LeadsTo_weaken)
+apply (blast intro: Always_LeadsToI subset_imp_LeadsTo)
+done
+
 
 end
 
