src/HOL/UNITY/Simple/Channel.thy
@@ -8,23 +8,65 @@ Unordered Channel
 From Misra, "A Logic for Concurrent Programming" (1994), section 13.3
 *)
 
-Channel = WFair +
+theory Channel = UNITY_Main:
 
-types state = nat set
+types state = "nat set"
 
 consts
-  F :: state program
+  F :: "state program"
 
 constdefs
-  minSet :: nat set => nat option
+  minSet :: "nat set => nat option"
     "minSet A == if A={} then None else Some (LEAST x. x:A)"
 
-rules
+axioms
 
-  UC1  "F : (minSet -` {Some x}) co (minSet -` (Some`atLeast x))"
+  UC1:  "F : (minSet -` {Some x}) co (minSet -` (Some`atLeast x))"
 
   (*  UC1  "F : {s. minSet s = x} co {s. x <= minSet s}"  *)
 
-  UC2  "F : (minSet -` {Some x}) leadsTo {s. x ~: s}"
+  UC2:  "F : (minSet -` {Some x}) leadsTo {s. x ~: s}"
+
+
+(*None represents "infinity" while Some represents proper integers*)
+lemma minSet_eq_SomeD: "minSet A = Some x ==> x : A"
+apply (unfold minSet_def)
+apply (simp split: split_if_asm)
+apply (fast intro: LeastI)
+done
+
+lemma minSet_empty [simp]: " minSet{} = None"
+by (unfold minSet_def, simp)
+
+lemma minSet_nonempty: "x:A ==> minSet A = Some (LEAST x. x: A)"
+by (unfold minSet_def, auto)
+
+lemma minSet_greaterThan:
+     "F : (minSet -` {Some x}) leadsTo (minSet -` (Some`greaterThan x))"
+apply (rule leadsTo_weaken)
+apply (rule_tac x1=x in psp [OF UC2 UC1], safe)
+apply (auto dest: minSet_eq_SomeD simp add: linorder_neq_iff)
+done
+
+(*The induction*)
+lemma Channel_progress_lemma:
+     "F : (UNIV-{{}}) leadsTo (minSet -` (Some`atLeast y))"
+apply (rule leadsTo_weaken_R)
+apply (rule_tac l = y and f = "the o minSet" and B = "{}" 
+       in greaterThan_bounded_induct, safe)
+apply (simp_all (no_asm_simp))
+apply (drule_tac [2] minSet_nonempty)
+ prefer 2 apply simp 
+apply (rule minSet_greaterThan [THEN leadsTo_weaken], safe)
+apply simp_all
+apply (drule minSet_nonempty, simp)
+done
+
+
+lemma Channel_progress: "!!y::nat. F : (UNIV-{{}}) leadsTo {s. y ~: s}"
+apply (rule Channel_progress_lemma [THEN leadsTo_weaken_R], clarify)
+apply (frule minSet_nonempty)
+apply (auto dest: Suc_le_lessD not_less_Least)
+done
 
 end
