src/HOL/UNITY/Simple/Common.thy
@@ -10,23 +10,96 @@ The state is identified with the one variable in existence.
 From Misra, "A Logic for Concurrent Programming" (1994), sections 5.1 and 13.1.
 *)
 
-Common = SubstAx + 
+theory Common = UNITY_Main:
 
 consts
-  ftime,gtime :: nat=>nat
+  ftime :: "nat=>nat"
+  gtime :: "nat=>nat"
 
-rules
-  fmono "m <= n ==> ftime m <= ftime n"
-  gmono "m <= n ==> gtime m <= gtime n"
+axioms
+  fmono: "m <= n ==> ftime m <= ftime n"
+  gmono: "m <= n ==> gtime m <= gtime n"
 
-  fasc  "m <= ftime n"
-  gasc  "m <= gtime n"
+  fasc:  "m <= ftime n"
+  gasc:  "m <= gtime n"
 
 constdefs
-  common :: nat set
+  common :: "nat set"
     "common == {n. ftime n = n & gtime n = n}"
 
-  maxfg :: nat => nat set
+  maxfg :: "nat => nat set"
     "maxfg m == {t. t <= max (ftime m) (gtime m)}"
+
+
+(*Misra's property CMT4: t exceeds no common meeting time*)
+lemma common_stable:
+     "[| ALL m. F : {m} Co (maxfg m); n: common |]  
+      ==> F : Stable (atMost n)"
+apply (drule_tac M = "{t. t<=n}" in Elimination_sing)
+apply (simp add: atMost_def Stable_def common_def maxfg_def le_max_iff_disj)
+apply (erule Constrains_weaken_R)
+apply (blast intro: order_eq_refl fmono gmono le_trans)
+done
+
+lemma common_safety:
+     "[| Init F <= atMost n;   
+         ALL m. F : {m} Co (maxfg m); n: common |]  
+      ==> F : Always (atMost n)"
+by (simp add: AlwaysI common_stable)
+
+
+(*** Some programs that implement the safety property above ***)
+
+lemma "SKIP : {m} co (maxfg m)"
+by (simp add: constrains_def maxfg_def le_max_iff_disj fasc)
+
+(*This one is  t := ftime t || t := gtime t*)
+lemma "mk_program (UNIV, {range(%t.(t,ftime t)), range(%t.(t,gtime t))}, UNIV)
+       : {m} co (maxfg m)"
+by (simp add: constrains_def maxfg_def le_max_iff_disj fasc)
+
+(*This one is  t := max (ftime t) (gtime t)*)
+lemma  "mk_program (UNIV, {range(%t.(t, max (ftime t) (gtime t)))}, UNIV)  
+       : {m} co (maxfg m)"
+by (simp add: constrains_def maxfg_def max_def gasc)
+
+(*This one is  t := t+1 if t <max (ftime t) (gtime t) *)
+lemma  "mk_program   
+          (UNIV, { {(t, Suc t) | t. t < max (ftime t) (gtime t)} }, UNIV)   
+       : {m} co (maxfg m)"
+by (simp add: constrains_def maxfg_def max_def gasc)
+
+
+(*It remans to prove that they satisfy CMT3': t does not decrease,
+  and that CMT3' implies that t stops changing once common(t) holds.*)
+
+
+(*** Progress under weak fairness ***)
+
+declare atMost_Int_atLeast [simp]
+
+lemma leadsTo_common_lemma:
+     "[| ALL m. F : {m} Co (maxfg m);  
+         ALL m: lessThan n. F : {m} LeadsTo (greaterThan m);  
+         n: common |]   
+      ==> F : (atMost n) LeadsTo common"
+apply (rule LeadsTo_weaken_R)
+apply (rule_tac f = id and l = n in GreaterThan_bounded_induct)
+apply (simp_all (no_asm_simp))
+apply (rule_tac [2] subset_refl)
+apply (blast dest: PSP_Stable2 intro: common_stable LeadsTo_weaken_R)
+done
+
+(*The "ALL m: -common" form echoes CMT6.*)
+lemma leadsTo_common:
+     "[| ALL m. F : {m} Co (maxfg m);  
+         ALL m: -common. F : {m} LeadsTo (greaterThan m);  
+         n: common |]   
+      ==> F : (atMost (LEAST n. n: common)) LeadsTo common"
+apply (rule leadsTo_common_lemma)
+apply (simp_all (no_asm_simp))
+apply (erule_tac [2] LeastI)
+apply (blast dest!: not_less_Least)
+done
 
 end
