src/HOL/UNITY/Simple/Deadlock.thy
@@ -1,1 +1,82 @@
-Deadlock = UNITY
+(*  Title:      HOL/UNITY/Deadlock
+    ID:         $Id$
+    Author:     Lawrence C Paulson, Cambridge University Computer Laboratory
+    Copyright   1998  University of Cambridge
+
+Deadlock examples from section 5.6 of 
+    Misra, "A Logic for Concurrent Programming", 1994
+*)
+
+theory Deadlock = UNITY:
+
+(*Trivial, two-process case*)
+lemma "[| F : (A Int B) co A;  F : (B Int A) co B |] ==> F : stable (A Int B)"
+by (unfold constrains_def stable_def, blast)
+
+
+(*a simplification step*)
+lemma Collect_le_Int_equals:
+     "(INT i: atMost n. A(Suc i) Int A i) = (INT i: atMost (Suc n). A i)"
+apply (induct_tac "n")
+apply (simp_all (no_asm_simp) add: atMost_Suc)
+apply auto
+done
+
+(*Dual of the required property.  Converse inclusion fails.*)
+lemma UN_Int_Compl_subset:
+     "(UN i: lessThan n. A i) Int (- A n) <=   
+      (UN i: lessThan n. (A i) Int (- A (Suc i)))"
+apply (induct_tac "n")
+apply (simp (no_asm_simp))
+apply (simp (no_asm) add: lessThan_Suc)
+apply blast
+done
+
+
+(*Converse inclusion fails.*)
+lemma INT_Un_Compl_subset:
+     "(INT i: lessThan n. -A i Un A (Suc i))  <=  
+      (INT i: lessThan n. -A i) Un A n"
+apply (induct_tac "n")
+apply (simp (no_asm_simp))
+apply (simp (no_asm_simp) add: lessThan_Suc)
+apply blast
+done
+
+
+(*Specialized rewriting*)
+lemma INT_le_equals_Int_lemma:
+     "A 0 Int (-(A n) Int (INT i: lessThan n. -A i Un A (Suc i))) = {}"
+by (blast intro: gr0I dest: INT_Un_Compl_subset [THEN subsetD])
+
+(*Reverse direction makes it harder to invoke the ind hyp*)
+lemma INT_le_equals_Int:
+     "(INT i: atMost n. A i) =  
+      A 0 Int (INT i: lessThan n. -A i Un A(Suc i))"
+apply (induct_tac "n", simp)
+apply (simp add: Int_ac Int_Un_distrib Int_Un_distrib2
+                 INT_le_equals_Int_lemma lessThan_Suc atMost_Suc)
+done
+
+lemma INT_le_Suc_equals_Int:
+     "(INT i: atMost (Suc n). A i) =  
+      A 0 Int (INT i: atMost n. -A i Un A(Suc i))"
+by (simp add: lessThan_Suc_atMost INT_le_equals_Int)
+
+
+(*The final deadlock example*)
+lemma
+  assumes zeroprem: "F : (A 0 Int A (Suc n)) co (A 0)"
+      and allprem:
+	    "!!i. i: atMost n ==> F : (A(Suc i) Int A i) co (-A i Un A(Suc i))"
+  shows "F : stable (INT i: atMost (Suc n). A i)"
+apply (unfold stable_def) 
+apply (rule constrains_Int [THEN constrains_weaken])
+   apply (rule zeroprem) 
+  apply (rule constrains_INT) 
+  apply (erule allprem)
+ apply (simp add: Collect_le_Int_equals Int_assoc INT_absorb)
+apply (simp add: INT_le_Suc_equals_Int)
+done
+
+end
