src/HOL/UNITY/Simple/Lift.thy
@@ -6,63 +6,63 @@
 The Lift-Control Example
 *)
 
-Lift = SubstAx +
+theory Lift = UNITY_Main:
 
 record state =
-  floor :: int		(*current position of the lift*)
-  open  :: bool		(*whether the door is open at floor*)
-  stop  :: bool		(*whether the lift is stopped at floor*)
-  req   :: int set	(*for each floor, whether the lift is requested*)
-  up    :: bool		(*current direction of movement*)
-  move  :: bool		(*whether moving takes precedence over opening*)
+  floor :: "int"	    (*current position of the lift*)
+  "open" :: "bool"	    (*whether the door is opened at floor*)
+  stop  :: "bool"	    (*whether the lift is stopped at floor*)
+  req   :: "int set"	    (*for each floor, whether the lift is requested*)
+  up    :: "bool"	    (*current direction of movement*)
+  move  :: "bool"	    (*whether moving takes precedence over opening*)
 
 consts
-  Min, Max :: int       (*least and greatest floors*)
+  Min :: "int"       (*least and greatest floors*)
+  Max :: "int"       (*least and greatest floors*)
 
-rules
-  Min_le_Max  "Min <= Max"
+axioms
+  Min_le_Max [iff]: "Min <= Max"
   
 constdefs
   
   (** Abbreviations: the "always" part **)
   
-  above :: state set
+  above :: "state set"
     "above == {s. EX i. floor s < i & i <= Max & i : req s}"
 
-  below :: state set
+  below :: "state set"
     "below == {s. EX i. Min <= i & i < floor s & i : req s}"
 
-  queueing :: state set
+  queueing :: "state set"
     "queueing == above Un below"
 
-  goingup :: state set
+  goingup :: "state set"
     "goingup   == above Int  ({s. up s}  Un -below)"
 
-  goingdown :: state set
+  goingdown :: "state set"
     "goingdown == below Int ({s. ~ up s} Un -above)"
 
-  ready :: state set
+  ready :: "state set"
     "ready == {s. stop s & ~ open s & move s}"
-
  
   (** Further abbreviations **)
 
-  moving :: state set
+  moving :: "state set"
     "moving ==  {s. ~ stop s & ~ open s}"
 
-  stopped :: state set
+  stopped :: "state set"
     "stopped == {s. stop s  & ~ open s & ~ move s}"
 
-  opened :: state set
+  opened :: "state set"
     "opened ==  {s. stop s  &  open s  &  move s}"
 
-  closed :: state set  (*but this is the same as ready!!*)
+  closed :: "state set"  (*but this is the same as ready!!*)
     "closed ==  {s. stop s  & ~ open s &  move s}"
 
-  atFloor :: int => state set
+  atFloor :: "int => state set"
     "atFloor n ==  {s. floor s = n}"
 
-  Req :: int => state set
+  Req :: "int => state set"
     "Req n ==  {s. n : req s}"
 
 
@@ -118,7 +118,7 @@ constdefs
 		        & Min <= n & n <= Max}"
 
 
-  Lift :: state program
+  Lift :: "state program"
     (*for the moment, we OMIT button_press*)
     "Lift == mk_program ({s. floor s = Min & ~ up s & move s & stop s &
 		          ~ open s & req s = {}},
@@ -129,27 +129,27 @@ constdefs
 
   (** Invariants **)
 
-  bounded :: state set
+  bounded :: "state set"
     "bounded == {s. Min <= floor s & floor s <= Max}"
 
-  open_stop :: state set
+  open_stop :: "state set"
     "open_stop == {s. open s --> stop s}"
   
-  open_move :: state set
+  open_move :: "state set"
     "open_move == {s. open s --> move s}"
   
-  stop_floor :: state set
+  stop_floor :: "state set"
     "stop_floor == {s. stop s & ~ move s --> floor s : req s}"
   
-  moving_up :: state set
+  moving_up :: "state set"
     "moving_up == {s. ~ stop s & up s -->
                    (EX f. floor s <= f & f <= Max & f : req s)}"
   
-  moving_down :: state set
+  moving_down :: "state set"
     "moving_down == {s. ~ stop s & ~ up s -->
                      (EX f. Min <= f & f <= floor s & f : req s)}"
   
-  metric :: [int,state] => int
+  metric :: "[int,state] => int"
     "metric ==
        %n s. if floor s < n then (if up s then n - floor s
 			          else (floor s - Min) + (n-Min))
@@ -158,12 +158,310 @@ constdefs
 		                  else floor s - n)
              else 0"
 
-locale floor =
-  fixes 
-    n	:: int
-  assumes
-    Min_le_n    "Min <= n"
-    n_le_Max    "n <= Max"
-  defines
+locale Floor =
+  fixes n
+  assumes Min_le_n [iff]: "Min <= n"
+      and n_le_Max [iff]: "n <= Max"
+
+lemma not_mem_distinct: "[| x ~: A;  y : A |] ==> x ~= y"
+by blast
+
+
+declare Lift_def [THEN def_prg_Init, simp]
+
+declare request_act_def [THEN def_act_simp, simp]
+declare open_act_def [THEN def_act_simp, simp]
+declare close_act_def [THEN def_act_simp, simp]
+declare req_up_def [THEN def_act_simp, simp]
+declare req_down_def [THEN def_act_simp, simp]
+declare move_up_def [THEN def_act_simp, simp]
+declare move_down_def [THEN def_act_simp, simp]
+declare button_press_def [THEN def_act_simp, simp]
+
+(*The ALWAYS properties*)
+declare above_def [THEN def_set_simp, simp]
+declare below_def [THEN def_set_simp, simp]
+declare queueing_def [THEN def_set_simp, simp]
+declare goingup_def [THEN def_set_simp, simp]
+declare goingdown_def [THEN def_set_simp, simp]
+declare ready_def [THEN def_set_simp, simp]
+
+(*Basic definitions*)
+declare bounded_def [simp] 
+        open_stop_def [simp] 
+        open_move_def [simp] 
+        stop_floor_def [simp]
+        moving_up_def [simp]
+        moving_down_def [simp]
+
+lemma open_stop: "Lift : Always open_stop"
+apply (rule AlwaysI, force) 
+apply (unfold Lift_def, constrains) 
+done
+
+lemma stop_floor: "Lift : Always stop_floor"
+apply (rule AlwaysI, force) 
+apply (unfold Lift_def, constrains)
+done
+
+(*This one needs open_stop, which was proved above*)
+lemma open_move: "Lift : Always open_move"
+apply (cut_tac open_stop)
+apply (rule AlwaysI, force) 
+apply (unfold Lift_def, constrains)
+done
+
+lemma moving_up: "Lift : Always moving_up"
+apply (rule AlwaysI, force) 
+apply (unfold Lift_def, constrains)
+apply (auto dest: zle_imp_zless_or_eq simp add: add1_zle_eq)
+done
+
+lemma moving_down: "Lift : Always moving_down"
+apply (rule AlwaysI, force) 
+apply (unfold Lift_def, constrains)
+apply (blast dest: zle_imp_zless_or_eq)
+done
+
+lemma bounded: "Lift : Always bounded"
+apply (cut_tac moving_up moving_down)
+apply (rule AlwaysI, force) 
+apply (unfold Lift_def, constrains, auto)
+apply (drule not_mem_distinct, assumption, arith)+
+done
+
+
+subsection{*Progress*}
+
+declare moving_def [THEN def_set_simp, simp]
+declare stopped_def [THEN def_set_simp, simp]
+declare opened_def [THEN def_set_simp, simp]
+declare closed_def [THEN def_set_simp, simp]
+declare atFloor_def [THEN def_set_simp, simp]
+declare Req_def [THEN def_set_simp, simp]
+
+
+(** The HUG'93 paper mistakenly omits the Req n from these! **)
+
+(** Lift_1 **)
+lemma E_thm01: "Lift : (stopped Int atFloor n) LeadsTo (opened Int atFloor n)"
+apply (cut_tac stop_floor)
+apply (unfold Lift_def, ensures_tac "open_act")
+done  (*lem_lift_1_5*)
+
+lemma E_thm02: "Lift : (Req n Int stopped - atFloor n) LeadsTo  
+                     (Req n Int opened - atFloor n)"
+apply (cut_tac stop_floor)
+apply (unfold Lift_def, ensures_tac "open_act")
+done  (*lem_lift_1_1*)
+
+lemma E_thm03: "Lift : (Req n Int opened - atFloor n) LeadsTo  
+                     (Req n Int closed - (atFloor n - queueing))"
+apply (unfold Lift_def, ensures_tac "close_act")
+done  (*lem_lift_1_2*)
+
+lemma E_thm04: "Lift : (Req n Int closed Int (atFloor n - queueing))   
+             LeadsTo (opened Int atFloor n)"
+apply (unfold Lift_def, ensures_tac "open_act")
+done  (*lem_lift_1_7*)
+
+
+(** Lift 2.  Statements of thm05a and thm05b were wrong! **)
+
+lemmas linorder_leI = linorder_not_less [THEN iffD1]
+
+lemmas (in Floor) le_MinD = Min_le_n [THEN order_antisym]
+              and Max_leD = n_le_Max [THEN [2] order_antisym]
+
+declare (in Floor) le_MinD [dest!]
+               and linorder_leI [THEN le_MinD, dest!]
+               and Max_leD [dest!]
+               and linorder_leI [THEN Max_leD, dest!]
+
+
+(*lem_lift_2_0 
+  NOT an ensures_tac property, but a mere inclusion
+  don't know why script lift_2.uni says ENSURES*)
+lemma (in Floor) E_thm05c: 
+    "Lift : (Req n Int closed - (atFloor n - queueing))    
+             LeadsTo ((closed Int goingup Int Req n)  Un  
+                      (closed Int goingdown Int Req n))"
+by (auto intro!: subset_imp_LeadsTo elim!: int_neqE)
+
+(*lift_2*)
+lemma (in Floor) lift_2: "Lift : (Req n Int closed - (atFloor n - queueing))    
+             LeadsTo (moving Int Req n)"
+apply (rule LeadsTo_Trans [OF E_thm05c LeadsTo_Un])
+apply (unfold Lift_def) 
+apply (ensures_tac [2] "req_down")
+apply (ensures_tac "req_up", auto)
+done
+
+
+(** Towards lift_4 ***)
+ 
+declare split_if_asm [split]
+
+
+(*lem_lift_4_1 *)
+lemma (in Floor) E_thm12a:
+     "0 < N ==>  
+      Lift : (moving Int Req n Int {s. metric n s = N} Int  
+              {s. floor s ~: req s} Int {s. up s})    
+             LeadsTo  
+               (moving Int Req n Int {s. metric n s < N})"
+apply (cut_tac moving_up)
+apply (unfold Lift_def, ensures_tac "move_up", safe)
+(*this step consolidates two formulae to the goal  metric n s' <= metric n s*)
+apply (erule linorder_leI [THEN order_antisym, symmetric])
+apply (auto simp add: metric_def)
+done
+
+
+(*lem_lift_4_3 *)
+lemma (in Floor) E_thm12b: "0 < N ==>  
+      Lift : (moving Int Req n Int {s. metric n s = N} Int  
+              {s. floor s ~: req s} - {s. up s})    
+             LeadsTo (moving Int Req n Int {s. metric n s < N})"
+apply (cut_tac moving_down)
+apply (unfold Lift_def, ensures_tac "move_down", safe)
+(*this step consolidates two formulae to the goal  metric n s' <= metric n s*)
+apply (erule linorder_leI [THEN order_antisym, symmetric])
+apply (auto simp add: metric_def)
+done
+
+(*lift_4*)
+lemma (in Floor) lift_4:
+     "0<N ==> Lift : (moving Int Req n Int {s. metric n s = N} Int  
+                            {s. floor s ~: req s}) LeadsTo      
+                           (moving Int Req n Int {s. metric n s < N})"
+apply (rule LeadsTo_Trans [OF subset_imp_LeadsTo
+                              LeadsTo_Un [OF E_thm12a E_thm12b]], auto)
+done
+
+
+(** towards lift_5 **)
+
+(*lem_lift_5_3*)
+lemma (in Floor) E_thm16a: "0<N    
+  ==> Lift : (closed Int Req n Int {s. metric n s = N} Int goingup) LeadsTo  
+             (moving Int Req n Int {s. metric n s < N})"
+apply (cut_tac bounded)
+apply (unfold Lift_def, ensures_tac "req_up")
+apply (auto simp add: metric_def)
+done
+
+
+(*lem_lift_5_1 has ~goingup instead of goingdown*)
+lemma (in Floor) E_thm16b: "0<N ==>    
+      Lift : (closed Int Req n Int {s. metric n s = N} Int goingdown) LeadsTo  
+                   (moving Int Req n Int {s. metric n s < N})"
+apply (cut_tac bounded)
+apply (unfold Lift_def, ensures_tac "req_down")
+apply (auto simp add: metric_def)
+done
+
+
+(*lem_lift_5_0 proves an intersection involving ~goingup and goingup,
+  i.e. the trivial disjunction, leading to an asymmetrical proof.*)
+lemma (in Floor) E_thm16c:
+     "0<N ==> Req n Int {s. metric n s = N} <= goingup Un goingdown"
+by (force simp add: metric_def)
+
+
+(*lift_5*)
+lemma (in Floor) lift_5:
+     "0<N ==> Lift : (closed Int Req n Int {s. metric n s = N}) LeadsTo    
+                     (moving Int Req n Int {s. metric n s < N})"
+apply (rule LeadsTo_Trans [OF subset_imp_LeadsTo
+                              LeadsTo_Un [OF E_thm16a E_thm16b]])
+apply (drule E_thm16c, auto)
+done
+
+
+(** towards lift_3 **)
+
+(*lemma used to prove lem_lift_3_1*)
+lemma (in Floor) metric_eq_0D [dest]:
+     "[| metric n s = 0;  Min <= floor s;  floor s <= Max |] ==> floor s = n"
+by (force simp add: metric_def)
+
+
+(*lem_lift_3_1*)
+lemma (in Floor) E_thm11: "Lift : (moving Int Req n Int {s. metric n s = 0}) LeadsTo    
+                       (stopped Int atFloor n)"
+apply (cut_tac bounded)
+apply (unfold Lift_def, ensures_tac "request_act", auto)
+done
+
+(*lem_lift_3_5*)
+lemma (in Floor) E_thm13: 
+  "Lift : (moving Int Req n Int {s. metric n s = N} Int {s. floor s : req s})  
+  LeadsTo (stopped Int Req n Int {s. metric n s = N} Int {s. floor s : req s})"
+apply (unfold Lift_def, ensures_tac "request_act")
+apply (auto simp add: metric_def)
+done
+
+(*lem_lift_3_6*)
+lemma (in Floor) E_thm14: "0 < N ==>  
+      Lift :  
+        (stopped Int Req n Int {s. metric n s = N} Int {s. floor s : req s})  
+        LeadsTo (opened Int Req n Int {s. metric n s = N})"
+apply (unfold Lift_def, ensures_tac "open_act")
+apply (auto simp add: metric_def)
+done
+
+(*lem_lift_3_7*)
+lemma (in Floor) E_thm15: "Lift : (opened Int Req n Int {s. metric n s = N})   
+             LeadsTo (closed Int Req n Int {s. metric n s = N})"
+apply (unfold Lift_def, ensures_tac "close_act")
+apply (auto simp add: metric_def)
+done
+
+
+(** the final steps **)
+
+lemma (in Floor) lift_3_Req: "0 < N ==>  
+      Lift :  
+        (moving Int Req n Int {s. metric n s = N} Int {s. floor s : req s})    
+        LeadsTo (moving Int Req n Int {s. metric n s < N})"
+apply (blast intro!: E_thm13 E_thm14 E_thm15 lift_5 intro: LeadsTo_Trans)
+done
+
+
+(*Now we observe that our integer metric is really a natural number*)
+lemma (in Floor) Always_nonneg: "Lift : Always {s. 0 <= metric n s}"
+apply (rule bounded [THEN Always_weaken])
+apply (auto simp add: metric_def)
+done
+
+lemmas (in Floor) R_thm11 = Always_LeadsTo_weaken [OF Always_nonneg E_thm11]
+
+lemma (in Floor) lift_3:
+     "Lift : (moving Int Req n) LeadsTo (stopped Int atFloor n)"
+apply (rule Always_nonneg [THEN integ_0_le_induct])
+apply (case_tac "0 < z")
+(*If z <= 0 then actually z = 0*)
+prefer 2 apply (force intro: R_thm11 order_antisym simp add: linorder_not_less)
+apply (rule LeadsTo_weaken_R [OF asm_rl Un_upper1])
+apply (rule LeadsTo_Trans [OF subset_imp_LeadsTo
+                              LeadsTo_Un [OF lift_4 lift_3_Req]], auto)
+done
+
+
+lemma (in Floor) lift_1: "Lift : (Req n) LeadsTo (opened Int atFloor n)"
+apply (rule LeadsTo_Trans)
+ prefer 2
+ apply (rule LeadsTo_Un [OF E_thm04 LeadsTo_Un_post])
+ apply (rule E_thm01 [THEN [2] LeadsTo_Trans_Un])
+ apply (rule lift_3 [THEN [2] LeadsTo_Trans_Un])
+ apply (rule lift_2 [THEN [2] LeadsTo_Trans_Un])
+ apply (rule LeadsTo_Trans_Un [OF E_thm02 E_thm03])
+apply (rule open_move [THEN Always_LeadsToI])
+apply (rule Always_LeadsToI [OF open_stop subset_imp_LeadsTo], clarify)
+(*The case split is not essential but makes the proof much faster.*)
+apply (case_tac "open x", auto)
+done
+
 
 end
