src/HOL/UNITY/Simple/Mutex.thy
@@ -6,7 +6,7 @@
 Based on "A Family of 2-Process Mutual Exclusion Algorithms" by J Misra
 *)
 
-Mutex = SubstAx +
+theory Mutex = UNITY_Main:
 
 record state =
   p :: bool
@@ -53,7 +53,7 @@ constdefs
   V4 :: command
     "V4 == {(s,s'). s' = s (|p:=False, n:=0|) & n s = 4}"
 
-  Mutex :: state program
+  Mutex :: "state program"
     "Mutex == mk_program ({s. ~ u s & ~ v s & m s = 0 & n s = 0},
 		 	  {U0, U1, U2, U3, U4, V0, V1, V2, V3, V4},
 			  UNIV)"
@@ -61,16 +61,166 @@ constdefs
 
   (** The correct invariants **)
 
-  IU :: state set
+  IU :: "state set"
     "IU == {s. (u s = (1 <= m s & m s <= 3)) & (m s = 3 --> ~ p s)}"
 
-  IV :: state set
+  IV :: "state set"
     "IV == {s. (v s = (1 <= n s & n s <= 3)) & (n s = 3 --> p s)}"
 
   (** The faulty invariant (for U alone) **)
 
-  bad_IU :: state set
+  bad_IU :: "state set"
     "bad_IU == {s. (u s = (1 <= m s & m s <= 3)) &
 	           (3 <= m s & m s <= 4 --> ~ p s)}"
+
+
+declare Mutex_def [THEN def_prg_Init, simp]
+
+declare U0_def [THEN def_act_simp, simp]
+declare U1_def [THEN def_act_simp, simp]
+declare U2_def [THEN def_act_simp, simp]
+declare U3_def [THEN def_act_simp, simp]
+declare U4_def [THEN def_act_simp, simp]
+declare V0_def [THEN def_act_simp, simp]
+declare V1_def [THEN def_act_simp, simp]
+declare V2_def [THEN def_act_simp, simp]
+declare V3_def [THEN def_act_simp, simp]
+declare V4_def [THEN def_act_simp, simp]
+
+declare IU_def [THEN def_set_simp, simp]
+declare IV_def [THEN def_set_simp, simp]
+declare bad_IU_def [THEN def_set_simp, simp]
+
+lemma IU: "Mutex : Always IU"
+apply (rule AlwaysI, force) 
+apply (unfold Mutex_def, constrains) 
+done
+
+
+lemma IV: "Mutex : Always IV"
+apply (rule AlwaysI, force) 
+apply (unfold Mutex_def, constrains)
+done
+
+(*The safety property: mutual exclusion*)
+lemma mutual_exclusion: "Mutex : Always {s. ~ (m s = 3 & n s = 3)}"
+apply (rule Always_weaken) 
+apply (rule Always_Int_I [OF IU IV], auto)
+done
+
+
+(*The bad invariant FAILS in V1*)
+lemma "Mutex : Always bad_IU"
+apply (rule AlwaysI, force) 
+apply (unfold Mutex_def, constrains, auto)
+(*Resulting state: n=1, p=false, m=4, u=false.  
+  Execution of V1 (the command of process v guarded by n=1) sets p:=true,
+  violating the invariant!*)
+oops
+
+
+lemma eq_123: "((1::int) <= i & i <= 3) = (i = 1 | i = 2 | i = 3)"
+by arith
+
+
+(*** Progress for U ***)
+
+lemma U_F0: "Mutex : {s. m s=2} Unless {s. m s=3}"
+by (unfold Unless_def Mutex_def, constrains)
+
+lemma U_F1: "Mutex : {s. m s=1} LeadsTo {s. p s = v s & m s = 2}"
+by (unfold Mutex_def, ensures_tac "U1")
+
+lemma U_F2: "Mutex : {s. ~ p s & m s = 2} LeadsTo {s. m s = 3}"
+apply (cut_tac IU)
+apply (unfold Mutex_def, ensures_tac U2)
+done
+
+lemma U_F3: "Mutex : {s. m s = 3} LeadsTo {s. p s}"
+apply (rule_tac B = "{s. m s = 4}" in LeadsTo_Trans)
+ apply (unfold Mutex_def)
+ apply (ensures_tac U3)
+apply (ensures_tac U4)
+done
+
+lemma U_lemma2: "Mutex : {s. m s = 2} LeadsTo {s. p s}"
+apply (rule LeadsTo_Diff [OF LeadsTo_weaken_L
+                             Int_lower2 [THEN subset_imp_LeadsTo]])
+apply (rule LeadsTo_Trans [OF U_F2 U_F3], auto)
+done
+
+lemma U_lemma1: "Mutex : {s. m s = 1} LeadsTo {s. p s}"
+by (rule LeadsTo_Trans [OF U_F1 [THEN LeadsTo_weaken_R] U_lemma2], blast)
+
+lemma U_lemma123: "Mutex : {s. 1 <= m s & m s <= 3} LeadsTo {s. p s}"
+by (simp add: eq_123 Collect_disj_eq LeadsTo_Un_distrib U_lemma1 U_lemma2 U_F3)
+
+(*Misra's F4*)
+lemma u_Leadsto_p: "Mutex : {s. u s} LeadsTo {s. p s}"
+by (rule Always_LeadsTo_weaken [OF IU U_lemma123], auto)
+
+
+(*** Progress for V ***)
+
+
+lemma V_F0: "Mutex : {s. n s=2} Unless {s. n s=3}"
+by (unfold Unless_def Mutex_def, constrains)
+
+lemma V_F1: "Mutex : {s. n s=1} LeadsTo {s. p s = (~ u s) & n s = 2}"
+by (unfold Mutex_def, ensures_tac "V1")
+
+lemma V_F2: "Mutex : {s. p s & n s = 2} LeadsTo {s. n s = 3}"
+apply (cut_tac IV)
+apply (unfold Mutex_def, ensures_tac "V2")
+done
+
+lemma V_F3: "Mutex : {s. n s = 3} LeadsTo {s. ~ p s}"
+apply (rule_tac B = "{s. n s = 4}" in LeadsTo_Trans)
+ apply (unfold Mutex_def)
+ apply (ensures_tac V3)
+apply (ensures_tac V4)
+done
+
+lemma V_lemma2: "Mutex : {s. n s = 2} LeadsTo {s. ~ p s}"
+apply (rule LeadsTo_Diff [OF LeadsTo_weaken_L
+                             Int_lower2 [THEN subset_imp_LeadsTo]])
+apply (rule LeadsTo_Trans [OF V_F2 V_F3], auto) 
+done
+
+lemma V_lemma1: "Mutex : {s. n s = 1} LeadsTo {s. ~ p s}"
+by (rule LeadsTo_Trans [OF V_F1 [THEN LeadsTo_weaken_R] V_lemma2], blast)
+
+lemma V_lemma123: "Mutex : {s. 1 <= n s & n s <= 3} LeadsTo {s. ~ p s}"
+by (simp add: eq_123 Collect_disj_eq LeadsTo_Un_distrib V_lemma1 V_lemma2 V_F3)
+
+
+(*Misra's F4*)
+lemma v_Leadsto_not_p: "Mutex : {s. v s} LeadsTo {s. ~ p s}"
+by (rule Always_LeadsTo_weaken [OF IV V_lemma123], auto)
+
+
+(** Absence of starvation **)
+
+(*Misra's F6*)
+lemma m1_Leadsto_3: "Mutex : {s. m s = 1} LeadsTo {s. m s = 3}"
+apply (rule LeadsTo_cancel2 [THEN LeadsTo_Un_duplicate])
+apply (rule_tac [2] U_F2)
+apply (simp add: Collect_conj_eq)
+apply (subst Un_commute)
+apply (rule LeadsTo_cancel2 [THEN LeadsTo_Un_duplicate])
+ apply (rule_tac [2] PSP_Unless [OF v_Leadsto_not_p U_F0])
+apply (rule U_F1 [THEN LeadsTo_weaken_R], auto)
+done
+
+(*The same for V*)
+lemma n1_Leadsto_3: "Mutex : {s. n s = 1} LeadsTo {s. n s = 3}"
+apply (rule LeadsTo_cancel2 [THEN LeadsTo_Un_duplicate])
+apply (rule_tac [2] V_F2)
+apply (simp add: Collect_conj_eq)
+apply (subst Un_commute)
+apply (rule LeadsTo_cancel2 [THEN LeadsTo_Un_duplicate])
+ apply (rule_tac [2] PSP_Unless [OF u_Leadsto_p V_F0])
+apply (rule V_F1 [THEN LeadsTo_weaken_R], auto)
+done
 
 end
