src/HOL/UNITY/Simple/Network.thy
@@ -8,7 +8,7 @@ The Communication Network
 From Misra, "A Logic for Concurrent Programming" (1994), section 5.7
 *)
 
-Network = UNITY +
+theory Network = UNITY:
 
 (*The state assigns a number to each process variable*)
 
@@ -17,5 +17,54 @@ datatype pvar = Sent | Rcvd | Idle
 datatype pname = Aproc | Bproc
 
 types state = "pname * pvar => nat"
+
+locale F_props =
+  fixes F 
+  assumes rsA: "F : stable {s. s(Bproc,Rcvd) <= s(Aproc,Sent)}"
+      and rsB: "F : stable {s. s(Aproc,Rcvd) <= s(Bproc,Sent)}"
+    and sent_nondec: "F : stable {s. m <= s(proc,Sent)}"
+    and rcvd_nondec: "F : stable {s. n <= s(proc,Rcvd)}"
+    and rcvd_idle: "F : {s. s(proc,Idle) = Suc 0 & s(proc,Rcvd) = m}
+                        co {s. s(proc,Rcvd) = m --> s(proc,Idle) = Suc 0}"
+    and sent_idle: "F : {s. s(proc,Idle) = Suc 0 & s(proc,Sent) = n}
+                        co {s. s(proc,Sent) = n}"
+  
+
+lemmas (in F_props) 
+        sent_nondec_A = sent_nondec [of _ Aproc]
+    and sent_nondec_B = sent_nondec [of _ Bproc]
+    and rcvd_nondec_A = rcvd_nondec [of _ Aproc]
+    and rcvd_nondec_B = rcvd_nondec [of _ Bproc]
+    and rcvd_idle_A = rcvd_idle [of Aproc]
+    and rcvd_idle_B = rcvd_idle [of Bproc]
+    and sent_idle_A = sent_idle [of Aproc]
+    and sent_idle_B = sent_idle [of Bproc]
+
+    and rs_AB = stable_Int [OF rsA rsB]
+    and sent_nondec_AB = stable_Int [OF sent_nondec_A sent_nondec_B]
+    and rcvd_nondec_AB = stable_Int [OF rcvd_nondec_A rcvd_nondec_B]
+    and rcvd_idle_AB = constrains_Int [OF rcvd_idle_A rcvd_idle_B]
+    and sent_idle_AB = constrains_Int [OF sent_idle_A sent_idle_B]
+    and nondec_AB = stable_Int [OF sent_nondec_AB rcvd_nondec_AB]
+    and idle_AB = constrains_Int [OF rcvd_idle_AB sent_idle_AB]
+    and nondec_idle = constrains_Int [OF nondec_AB [unfolded stable_def] 
+                                         idle_AB]
+
+lemma (in F_props)
+  shows "F : stable {s. s(Aproc,Idle) = Suc 0 & s(Bproc,Idle) = Suc 0 &  
+			s(Aproc,Sent) = s(Bproc,Rcvd) &  
+			s(Bproc,Sent) = s(Aproc,Rcvd) &  
+			s(Aproc,Rcvd) = m & s(Bproc,Rcvd) = n}"
+apply (unfold stable_def) 
+apply (rule constrainsI)
+apply (drule constrains_Int [OF rs_AB [unfolded stable_def] nondec_idle, 
+                             THEN constrainsD], assumption)
+apply simp_all
+apply (blast intro!: order_refl del: le0, clarify) 
+apply (subgoal_tac "s' (Aproc, Rcvd) = s (Aproc, Rcvd)")
+apply (subgoal_tac "s' (Bproc, Rcvd) = s (Bproc, Rcvd)") 
+apply simp 
+apply (blast intro: order_antisym le_trans eq_imp_le)+
+done
 
 end
